feat: prove forM_invariant_lemma

src/SelectionSort.thy
@@ -2,6 +2,74 @@ theory SelectionSort
   imports Main MVector
 begin
 
+primrec snoc :: "'a list \<Rightarrow> 'a \<Rightarrow> 'a list" where
+  "snoc [] x = [x]"
+| "snoc (y#ys) x = y # snoc ys x"
+
+lemma snoc_length: "length (snoc ys y) = Suc (length ys)"
+  by (induct ys, auto)
+
+lemma snoc_take_init: "take (size ys) (snoc ys y) = ys"
+  by (induct ys, auto)
+
+lemma snoc_take_all: "take (size ys + 1) (snoc ys y) = (snoc ys y)"
+  by (induct ys, auto)
+
+lemma snoc_induct:
+  assumes "P []"
+  and "\<And>xs y. P xs \<Longrightarrow> P (snoc xs y)"
+  shows "P xs"
+  apply (induct "size xs" arbitrary: xs)
+  apply (simp add: assms(1))
+proof-
+  have cons_snoc: "\<And>(a :: 'a list) x xs. a = x # xs \<Longrightarrow> \<exists>y ys. a = snoc ys y"
+  proof-
+    fix a :: "'a list" and x xs
+    show cons_snoc: "a = x # xs \<Longrightarrow> \<exists>y ys. a = snoc ys y"
+      apply (induct a arbitrary: x xs, auto)
+    proof-
+      fix x :: 'a and xs
+      assume "\<And>x (xsa :: 'a list). xs = x # xsa \<Longrightarrow> \<exists>y ys. x # xsa = snoc ys y"
+      show "\<exists>y ys. x # xs = snoc ys y"
+        apply (cases xs)
+        apply (metis snoc.simps(1))
+        by (metis \<open>\<And>xsa xa. xs = xa # xsa \<Longrightarrow> \<exists>y ys. xa # xsa = snoc ys y\<close> snoc.simps(2))
+    qed
+  qed
+
+  fix x and xs :: "'a list"
+  assume "\<And>xs. x = length xs \<Longrightarrow> P xs"
+  and "Suc x = length xs"
+  obtain y ys where "xs = y # ys"
+    by (meson Suc_length_conv \<open>Suc x = length xs\<close>)
+  then obtain z zs where "xs = snoc zs z"
+    using cons_snoc by blast
+  hence "x = length zs"
+    by (simp add: Suc_inject \<open>Suc x = length xs\<close> snoc_length)
+  show "P xs"
+    by (simp add: \<open>\<And>xs. x = length xs \<Longrightarrow> P xs\<close> \<open>x = length zs\<close> \<open>xs = snoc zs z\<close> assms(2))
+qed
+
+lemma forM_invariant:
+  assumes "P 0 ((),h)"
+  and "\<And>i xs h. \<lbrakk> P i (execute (forMu (take i xs) program) h); i < size xs \<rbrakk> \<Longrightarrow> P (i+1) (execute (forMu (take (i+1) xs) program) h)"
+  shows "P (size xs) (execute (forMu xs program) h)"
+  apply (induct xs rule: snoc_induct)
+  apply (simp add: return_def assms(1))
+proof-
+  fix xs :: "'a list" and y
+  have "length xs < length (snoc xs y)"
+    by (simp add: snoc_length)
+
+  assume "P (length xs) (execute (forMu xs program) h)"
+  hence "P (length xs) (execute (forMu (take (length xs) (snoc xs y)) program) h)"
+    by (simp add: snoc_take_init)
+  have "P (length (snoc xs y)) (execute (forMu (take (length (snoc xs y)) (snoc xs y)) program) h)"
+    by (metis Suc_eq_plus1 \<open>P (length xs) (execute (forMu (take (length xs) (snoc xs y)) program) h)\<close> assms(2) lessI snoc_length)
+  thus "P (length (snoc xs y)) (execute (forMu (snoc xs y) program) h)"
+    by simp
+qed
+
 definition selection_sort :: "nat mvector \<Rightarrow> unit io" where
   "selection_sort arr = (let n = size_of_mvector arr in forMu [0..<n] (\<lambda>i. do {
     min_ref \<leftarrow> ref i;
@@ -45,22 +113,16 @@ lemma selection_sort_as_outer_loop: "selection_sort arr = (let n = size_of_mvect
   unfolding selection_sort_def outer_loop_def
   by simp
 
-lemma forM_invariant:
-  assumes "P 0 ((),h)"
-  and "\<And>i h. \<lbrakk> P i (execute (forMu (take i xs) program) h); i < size xs \<rbrakk> \<Longrightarrow> P (i+1) (execute (forMu (take (i+1) xs) program) h)"
-  shows "P (size xs) (execute (forMu xs program) h)"
-  sorry
-
 definition is_sorted_outer where
   "is_sorted_outer mvec i n h = (case execute (forMu [0..<i] (outer_loop mvec n)) h of (_,h') \<Rightarrow> sorted (take i (get_over mvec h')))"
 
 lemma outer_loop_invariant:
   assumes "n = size_of_mvector arr"
-  and "\<And>i. is_sorted_outer arr i n h \<Longrightarrow> is_sorted_outer arr (i+1) n h"
+  and "\<And>i n. is_sorted_outer arr i n h \<Longrightarrow> is_sorted_outer arr (i+1) n h"
   shows "is_sorted_outer arr n n h"
   apply (simp add: is_sorted_outer_def)
-  using forM_invariant [of "\<lambda>i _. is_sorted_outer arr i n h" _ "[0..<n]"]
-  using assms(2) is_sorted_outer_def by force
+  using forM_invariant [of "\<lambda>i _. is_sorted_outer arr i n h"]
+  by (metis (mono_tags, lifting) SelectionSort.sorted.simps(1) assms(2) diff_zero is_sorted_outer_def length_upt split_def take0)
 
 theorem selection_sort_is_sorted:
   assumes "effect (selection_sort_program xs) h h' rs"
@@ -79,7 +141,7 @@ proof-
   hence "\<And>h. take (size xs) (get_over arr h) = get_over arr h"
     by simp
 
-  have "\<And>i. is_sorted_outer arr i (size xs) h' \<Longrightarrow> is_sorted_outer arr (i+1) (size xs) h'"
+  have "\<And>i n. is_sorted_outer arr i n h' \<Longrightarrow> is_sorted_outer arr (i+1) n h'"
     sorry
 
   hence "is_sorted_outer arr (size xs) (size xs) h'"
